cedar-lean/Cedar/Thm/Validation/Levels/GetAttr.lean
@@ -35,15 +35,14 @@ open Cedar.Data
 open Cedar.Spec
 open Cedar.Validation
 
-theorem level_based_slicing_is_sound_get_attr_entity {e : Expr} {tx₁: TypedExpr} {ty : CedarType} {a : Attr} {n : Nat} {c₀ c₁: Capabilities} {env : TypeEnv} {request : Request} {entities slice : Entities}
-  (hs : slice = entities.sliceAtLevel request n)
+theorem level_based_slicing_is_sound_get_attr_entity {e : Expr} {tx₁: TypedExpr} {ty : CedarType} {a : Attr} {n : Nat} {c₀ c₁: Capabilities} {env : TypeEnv} {request : Request} {entities : Entities}
   (hc : CapabilitiesInvariant c₀ request entities)
   (hr : InstanceOfWellFormedEnvironment request entities env)
   (hl : (tx₁.getAttr a ty).AtLevel env n)
   (ht : typeOf e c₀ env = Except.ok (tx₁, c₁))
   (hety : tx₁.typeOf = CedarType.entity ety)
   (ihe : TypedAtLevelIsSound e)
-  : evaluate (.getAttr e a) request entities = evaluate (.getAttr e a) request slice
+  : evaluate (.getAttr e a) request entities = evaluate (.getAttr e a) request (entities.sliceAtLevel request n)
 := by
   have ⟨ hgc, v, he, hv ⟩ := type_of_is_sound hc hr ht
   rw [hety] at hv
@@ -56,28 +55,27 @@ theorem level_based_slicing_is_sound_get_attr_entity {e : Expr} {tx₁: TypedExp
   rename_i n hel₁ hl₁ _
   simp only [evaluate]
   have hl₁' := entity_access_at_level_then_at_level hl₁
-  specialize ihe hs hc hr ht hl₁'
+  specialize ihe hc hr ht hl₁'
   rw [←ihe]
   unfold EvaluatesTo at he
   rcases he with he | he | he | he <;> simp only [he, Except.bind_err]
-  have hfeq := checked_eval_entity_find_entities_eq_find_slice hc hr ht hl₁ he hs
+  have hfeq := checked_eval_entity_find_entities_eq_find_slice hc hr ht hl₁ he
   simp [hfeq, getAttr, attrsOf, Entities.attrs, Map.findOrErr]
 
-theorem level_based_slicing_is_sound_get_attr_record {e : Expr} {tx : TypedExpr} {ty : CedarType} {a : Attr} {n : Nat} {c₀: Capabilities} {env : TypeEnv} {request : Request} {entities slice : Entities}
-  (hs : slice = entities.sliceAtLevel request n)
+theorem level_based_slicing_is_sound_get_attr_record {e : Expr} {tx : TypedExpr} {ty : CedarType} {a : Attr} {n : Nat} {c₀: Capabilities} {env : TypeEnv} {request : Request} {entities : Entities}
   (hc : CapabilitiesInvariant c₀ request entities)
   (hr : InstanceOfWellFormedEnvironment request entities env)
   (hl : (tx.getAttr a ty).AtLevel env n)
   (htx : typeOf e c₀ env = Except.ok (tx, c₁'))
   (hrty : tx.typeOf = CedarType.record rty)
   (ihe : TypedAtLevelIsSound e)
-  : evaluate (.getAttr e a) request entities = evaluate (.getAttr e a) request slice
+  : evaluate (.getAttr e a) request entities = evaluate (.getAttr e a) request (entities.sliceAtLevel request n)
 := by
   cases hl
   case getAttr hety =>
     simp [hety] at hrty
   rename_i hl
-  have ih := ihe hs hc hr htx hl
+  have ih := ihe hc hr htx hl
   simp only [evaluate, ←ih]
   cases he₁ : evaluate e request entities <;> simp only [Except.bind_err, Except.bind_ok]
   rename_i v
@@ -89,21 +87,20 @@ theorem level_based_slicing_is_sound_get_attr_record {e : Expr} {tx : TypedExpr}
     simpa [EvaluatesTo, hv, he₁] using he
   simp [he, getAttr, attrsOf]
 
-theorem level_based_slicing_is_sound_get_attr {e : Expr} {tx : TypedExpr} {a : Attr} {n : Nat} {c₀ c₁: Capabilities} {env : TypeEnv} {request : Request} {entities slice : Entities}
-  (hs : slice = entities.sliceAtLevel request n)
+theorem level_based_slicing_is_sound_get_attr {e : Expr} {tx : TypedExpr} {a : Attr} {n : Nat} {c₀ c₁: Capabilities} {env : TypeEnv} {request : Request} {entities : Entities}
   (hc : CapabilitiesInvariant c₀ request entities)
   (hr : InstanceOfWellFormedEnvironment request entities env)
   (ht : typeOf (e.getAttr a) c₀ env = Except.ok (tx, c₁))
   (hl : tx.AtLevel env n)
   (ihe : TypedAtLevelIsSound e)
-  : evaluate (.getAttr e a) request entities = evaluate (.getAttr e a) request slice
+  : evaluate (.getAttr e a) request entities = evaluate (.getAttr e a) request (entities.sliceAtLevel request n)
 := by
   have ⟨ h₇, ty₁, _, ht, h₅, h₆ ⟩ := type_of_getAttr_inversion ht
   rw [h₅] at hl
   cases h₆
   case _ hety =>
     replace ⟨ ety, hety ⟩ := hety
-    exact level_based_slicing_is_sound_get_attr_entity hs hc hr hl ht hety ihe
+    exact level_based_slicing_is_sound_get_attr_entity hc hr hl ht hety ihe
   case _ hrty =>
     replace ⟨ rty, hrty ⟩ := hrty
-    exact level_based_slicing_is_sound_get_attr_record hs hc hr hl ht hrty ihe
+    exact level_based_slicing_is_sound_get_attr_record hc hr hl ht hrty ihe
